Accum Wasm type list in codegen; fix call_indirect

theories/compiler/codegen.v
@@ -5,7 +5,7 @@ Local Open Scope program_scope.
 
 Require Import stdpp.list_monad.
 
-From ExtLib.Data Require Import List.
+From ExtLib.Data Require Import List PPair.
 From ExtLib.Data.Monads Require Import EitherMonad StateMonad WriterMonad.
 From ExtLib.Structures Require Import Monoid Monads.
 
@@ -16,19 +16,28 @@ From RichWasm.compiler Require Import prelude accum.
 
 Module W := Wasm.datatypes.
 
-Notation wlocal_ctx := (list W.value_type) (only parsing).
+Definition wtype_ctx : Type := list W.function_type.
 
-Definition codegen : Type -> Type := accumT (list W.value_type) (writerT W.expr (sum error)).
+Definition wlocal_ctx : Type := list W.value_type.
 
-Definition run_codegen {A : Type} (c : codegen A) (wl : wlocal_ctx) : error + A * wlocal_ctx * W.expr :=
-  match runWriterT (runAccumT c wl) with
+Definition codegen : Type -> Type := accumT (wtype_ctx * wlocal_ctx) (writerT W.expr (sum error)).
+
+Definition run_codegen {A : Type} (c : codegen A) (wt : wtype_ctx) (wl : wlocal_ctx) :
+  error + A * wtype_ctx * wlocal_ctx * W.expr :=
+  match runWriterT (runAccumT c (wt, wl)) with
   | inl e => inl e
-  | inr x => inr (PPair.pfst x, PPair.psnd x)
+  | inr x => inr (x.(pfst).1, x.(pfst).2.1, x.(pfst).2.2, x.(psnd))
   end.
 
-Definition wlalloc (fe : function_env) (ty : W.value_type) : codegen W.localidx :=
-  wl ← get;
-  acc [ty];;
+(* TODO: Check if the type is already in the list. *)
+Definition wtinsert (tf : W.function_type) : codegen W.typeidx :=
+  '(wt, _) ← get;
+  acc ([tf], []);;
+  ret (W.Mk_typeidx (length wt)).
+
+Definition wlalloc (fe : function_env) (t : W.value_type) : codegen W.localidx :=
+  '(_, wl) ← get;
+  acc ([], [t]);;
   ret (W.Mk_localidx (fe_wlocal_offset fe + length wl)).
 
 Definition emit (e : W.basic_instruction) : codegen unit := tell [e].
@@ -104,10 +113,10 @@ Lemma runWriterT_sum_bind_dist {A B L E}
   (f : A -> writerT L (sum E) B)
   (x : B)
   (l : L) :
-  runWriterT (c ≫= f) = inr (PPair.ppair x l) ->
+  runWriterT (c ≫= f) = inr (ppair x l) ->
   exists x1 l1 l2,
-  runWriterT c = inr (PPair.ppair x1 l1) /\
-  runWriterT (f x1) = inr (PPair.ppair x l2) /\
+  runWriterT c = inr (ppair x1 l1) /\
+  runWriterT (f x1) = inr (ppair x l2) /\
   l = monoid_plus l1 l2.
 Proof.
   intros H.
@@ -115,13 +124,13 @@ Proof.
   destruct c.
   cbn in H.
   destruct runWriterT; first congruence.
-  exists (PPair.pfst p).
-  exists (PPair.psnd p).
-  destruct (f (PPair.pfst p)).
+  exists p.(pfst).
+  exists p.(psnd).
+  destruct (f p.(pfst)).
   cbn in H.
   destruct runWriterT; first congruence.
   cbn.
-  exists (PPair.psnd p0).
+  exists p0.(psnd).
   split; first reflexivity.
   split.
   - inversion H. reflexivity.
@@ -137,10 +146,10 @@ Lemma runWriterT_runAccumT_sum_bind_dist {E L S A B}
   (s s' : S)
   (l : L)
   (x : B) :
-  runWriterT (runAccumT (c ≫= f) s) = inr (PPair.ppair (x, s') l) ->
+  runWriterT (runAccumT (c ≫= f) s) = inr (ppair (x, s') l) ->
   exists x1 s1 s2 l1 l2,
-  runWriterT (runAccumT c s) = inr (PPair.ppair (x1, s1) l1) /\
-  runWriterT (runAccumT (f x1) (monoid_plus s s1)) = inr (PPair.ppair (x, s2) l2) /\
+  runWriterT (runAccumT c s) = inr (ppair (x1, s1) l1) /\
+  runWriterT (runAccumT (f x1) (monoid_plus s s1)) = inr (ppair (x, s2) l2) /\
   s' = monoid_plus s1 s2 /\
   l = monoid_plus l1 l2.
 Proof.
@@ -161,22 +170,23 @@ Proof.
   - auto.
 Qed.
 
-Lemma run_codegen_def {A} (c : codegen A) wl wl' x es:
-  run_codegen c wl = inr (x, wl', es) <->
-  runWriterT (runAccumT c wl) = inr (PPair.ppair (x, wl') es).
+Lemma run_codegen_def {A} (c : codegen A) wt wt' wl wl' x es:
+  run_codegen c wt wl = inr (x, wt', wl', es) <->
+  runWriterT (runAccumT c (wt, wl)) = inr (ppair (x, (wt', wl')) es).
 Proof.
   split.
   {
     intros H.
     unfold run_codegen in H.
-    destruct (runWriterT (runAccumT c wl)); first congruence.
+    destruct (runWriterT (runAccumT c (wt, wl))); first congruence.
     inversion H.
+    destruct p. destruct pfst. destruct p.
     reflexivity.
   }
   {
     intros H.
     unfold run_codegen.
-    destruct (runWriterT (runAccumT c wl)); first congruence.
+    destruct (runWriterT (runAccumT c (wt, wl))); first congruence.
     inversion H.
     reflexivity.
   }
@@ -193,39 +203,37 @@ Proof.
     apply app_nil_r.
 Qed.
 
-Lemma run_codegen_bind_dist {A B} (c : codegen A) (f : A -> codegen B) wl wl' es x :
-  run_codegen (c ≫= f) wl = inr (x, wl', es) ->
-  exists x1 wl1 wl2 es1 es2,
-  run_codegen c wl = inr (x1, wl1, es1) /\
-  run_codegen (f x1) (wl ++ wl1) = inr (x, wl2, es2) /\
-  wl' = wl1 ++ wl2 /\
-  es = es1 ++ es2.
+Lemma run_codegen_bind_dist {A B} (c : codegen A) (f : A -> codegen B) wt wt' wl wl' es x :
+  run_codegen (c ≫= f) wt wl = inr (x, wt', wl', es) ->
+  exists x1 wt1 wt2 wl1 wl2 es1 es2,
+    run_codegen c wt wl = inr (x1, wt1, wl1, es1) /\
+      run_codegen (f x1) (wt ++ wt1) (wl ++ wl1) = inr (x, wt2, wl2, es2) /\
+      wt' = wt1 ++ wt2 /\
+      wl' = wl1 ++ wl2 /\
+      es = es1 ++ es2.
 Proof.
   intros H.
   rewrite run_codegen_def in H.
   apply runWriterT_runAccumT_sum_bind_dist in H; [|by typeclasses eauto].
-  destruct H as (x1 & s1 & s2 & l1 & l2 & H1 & H2 & Hwl' & Hes).
-  exists x1, s1, s2, l1, l2.
+  destruct H as (x1 & [wt1 wl1] & [wt2 wl2] & l1 & l2 & H1 & H2 & Hwl' & Hes).
+  inversion Hwl'.
+  exists x1, wt1, wt2, wl1, wl2, l1, l2.
   rewrite !run_codegen_def.
-  split; [|split; [|split]].
-  - assumption.
-  - assumption.
-  - assumption.
-  - assumption.
+  repeat split; assumption.
 Qed.
 
-Lemma run_codegen_try_option_inr {A} (c: option A) e x wl wl' es :
-  run_codegen (try_option e c) wl = inr (x, wl', es) ->
-  c = Some x /\ wl' = [] /\ es = [].
+Lemma run_codegen_try_option_inr {A} (c: option A) e x wt wt' wl wl' es :
+  run_codegen (try_option e c) wt wl = inr (x, wt', wl', es) ->
+  c = Some x /\ wt' = [] /\ wl' = [] /\ es = [].
 Proof.
   intros H.
   destruct c; cbn in H; [|congruence].
   inversion H; auto.
 Qed.
 
-Lemma run_codegen_capture {A} (c : codegen A) (wl wl': wlocal_ctx) es es' x :
-  run_codegen (capture c) wl = inr (x, es', wl', es) ->
-  run_codegen c wl = inr (x, wl', es') /\ es = [].
+Lemma run_codegen_capture {A} (c : codegen A) wt wt' wl wl' es es' x :
+  run_codegen (capture c) wt wl = inr (x, es', wt', wl', es) ->
+  run_codegen c wt wl = inr (x, wt', wl', es') /\ es = [].
 Proof.
   intros H.
   unfold run_codegen.
@@ -236,44 +244,47 @@ Proof.
   cbn in H.
   unfold run_codegen in *.
   cbn in H.
-  destruct (runWriterT (runAccumT c wl)); first congruence.
+  destruct (runWriterT (runAccumT c (wt, wl))); first congruence.
   cbn in H.
   destruct p.
   cbn in *.
   destruct pfst.
   cbn in H.
   inversion H.
-  subst a psnd wl' es.
+  subst a psnd wt' wl' es.
   clear H.
-  rewrite app_nil_r.
+  destruct p.
+  rewrite !app_nil_r.
   split; reflexivity.
 Qed.
 
-Lemma run_codegen_ret {A} (a: A) wl wl' x es :
-  run_codegen (mret a) wl = inr (x, wl', es) ->
-  x = a /\ wl' = [] /\ es = [].
+Lemma run_codegen_ret {A} (a : A) wt wt' wl wl' x es :
+  run_codegen (mret a) wt wl = inr (x, wt', wl', es) ->
+  x = a /\ wt' = [] /\ wl' = [] /\ es = [].
 Proof.
   intros Hret.
   inversion Hret.
   auto.
 Qed.
 
-Lemma run_codegen_emit wl e x wl' es' :
-  run_codegen (emit e) wl = inr (x, wl', es') ->
+Lemma run_codegen_emit wt wl e x wt' wl' es' :
+  run_codegen (emit e) wt wl = inr (x, wt', wl', es') ->
   x = tt /\
-  wl' = [] /\
-  es' = [e].
+    wt' = [] /\
+    wl' = [] /\
+    es' = [e].
 Proof.
   intros Hemit.
   inversion Hemit.
   auto.
 Qed.
 
-Lemma run_codegen_emit_all wl es x wl' es' :
-  run_codegen (emit_all es) wl = inr (x, wl', es') ->
+Lemma run_codegen_emit_all wt wl es x wt' wl' es' :
+  run_codegen (emit_all es) wt wl = inr (x, wt', wl', es') ->
   x = tt /\
-  wl' = [] /\
-  es' = es.
+    wt' = [] /\
+    wl' = [] /\
+    es' = es.
 Proof.
   intros Hemit.
   inversion Hemit.
@@ -283,50 +294,55 @@ Qed.
 
 Ltac inv_cg_try_option Hrun :=
   let Heq1 := fresh "Heq_some" in
-  let Heq2 := fresh "Heq_wl" in
-  let Heq3 := fresh "Heq_nil" in
+  let Heq2 := fresh "Heq_wt" in
+  let Heq3 := fresh "Heq_wl" in
+  let Heq4 := fresh "Heq_nil" in
   apply run_codegen_try_option_inr in Hrun;
-  destruct Hrun as (Heq1 & Heq2 & Heq3);
-  rewrite ?Heq1, ?Heq2, ?Heq3 in *.
+  destruct Hrun as (Heq1 & Heq2 & Heq3 & Heq4);
+  rewrite ?Heq1, ?Heq2, ?Heq3, ?Heq4 in *.
 
-Ltac inv_cg_bind Hbind res wl1 wl2 es1 es2 Hcg1 Hcg2 :=
+Ltac inv_cg_bind Hbind res wt1 wt2 wl1 wl2 es1 es2 Hcg1 Hcg2 :=
+  let Hwteq := fresh "Hwt_app_eq" in
   let Hwleq := fresh "Hwl_app_eq" in
   let Heseq := fresh "Hes_app_eq" in
   apply run_codegen_bind_dist in Hbind;
-  destruct Hbind as (res & wl1 & wl2 & es1 & es2 & Hcg1 & Hcg2 & Hwleq & Heseq);
-  rewrite Heseq, Hwleq.
+  destruct Hbind as (res & wt1 & wt2 & wl1 & wl2 & es1 & es2 & Hcg1 & Hcg2 & Hwteq & Hwleq & Heseq);
+  rewrite ?Heseq, ?Hwteq, ?Hwleq in *.
 
 Ltac inv_cg_ret Hret :=
   let Hretval := fresh "Hretval" in
+  let Hwt := fresh "Hwt" in
   let Hwl := fresh "Hwl" in
   let Hes := fresh "Hes" in
   apply run_codegen_ret in Hret;
-  destruct Hret as (Hretval & Hwl & Hes);
-  rewrite ?Hretval, ?Hwl, ?Hes in *.
+  destruct Hret as (Hretval & Hwt & Hwl & Hes);
+  rewrite ?Hretval, ?Hwt, ?Hwl, ?Hes in *.
 
 Ltac inv_cg_emit Hemit :=
   let Hretval := fresh "Hretval" in
+  let Hwt := fresh "Hwt" in
   let Hwl := fresh "Hwl" in
   let Hes := fresh "Hes" in
   apply run_codegen_emit in Hemit;
-  destruct Hemit as (Hretval & Hwl & Hes);
-  rewrite ?Hretval, ?Hwl, ?Hes in *.
+  destruct Hemit as (Hretval & Hwt & Hwl & Hes);
+  rewrite ?Hretval, ?Hwt, ?Hwl, ?Hes in *.
 
 Ltac inv_cg_emit_all Hemit :=
   let Hretval := fresh "Hretval" in
+  let Hwt := fresh "Hwt" in
   let Hwl := fresh "Hwl" in
   let Hes := fresh "Hes" in
   apply run_codegen_emit_all in Hemit;
-  destruct Hemit as (Hretval & Hwl & Hes);
-  rewrite ?Hretval, ?Hwl, ?Hes in *.
+  destruct Hemit as (Hretval & Hwt & Hwl & Hes);
+  rewrite ?Hretval, ?Hwt, ?Hwl, ?Hes in *.
 
-Example emit_ret_test wl x y z :
+Example emit_ret_test wt wl w x y z :
   run_codegen (emit W.BI_nop;;
-               mret 7) wl = inr (x, y, z) ->
-  x = 7 /\ y = [] /\ z = [W.BI_nop].
+               mret 7) wt wl = inr (w, x, y, z) ->
+  w = 7 /\ x = [] /\ y = [] /\ z = [W.BI_nop].
 Proof.
   intros Hrun.
-  inv_cg_bind Hrun res wl1 wl2 es1 es2 Hemit Hret.
+  inv_cg_bind Hrun res wt1 wt2 wl1 wl2 es1 es2 Hemit Hret.
   inv_cg_emit Hemit.
   inv_cg_ret Hret.
   rewrite app_nil_r.
